pulse/share/pulse/examples/by-example/PulseTutorial.ImplicationAndForall.fst
@@ -1,3 +1,19 @@
+(*
+   Copyright 2023 Microsoft Research
+
+   Licensed under the Apache License, Version 2.0 (the "License");
+   you may not use this file except in compliance with the License.
+   You may obtain a copy of the License at
+
+       http://www.apache.org/licenses/LICENSE-2.0
+
+   Unless required by applicable law or agreed to in writing, software
+   distributed under the License is distributed on an "AS IS" BASIS,
+   WITHOUT WARRANTIES OR CONDITIONS OF ANY KIND, either express or implied.
+   See the License for the specific language governing permissions and
+   limitations under the License.
+*)
+
 module PulseTutorial.ImplicationAndForall
 open Pulse.Lib.Pervasives
 open Pulse.Lib.Stick.Util
@@ -8,7 +24,7 @@ open GR
 
 //regain_half$
 let regain_half #a (x:GR.ref a) (v:a) =
-  pts_to x #one_half v @==> pts_to x v
+  pts_to x #0.5R v @==> pts_to x v
 //regain_half$
 
 
@@ -16,11 +32,11 @@ let regain_half #a (x:GR.ref a) (v:a) =
 ghost 
 fn intro_regain_half (x:GR.ref int)
 requires pts_to x 'v
-ensures pts_to x #one_half 'v ** regain_half x 'v
+ensures pts_to x #0.5R 'v ** regain_half x 'v
 {
   ghost
   fn aux ()
-  requires pts_to x #one_half 'v ** pts_to x #one_half 'v
+  requires pts_to x #0.5R 'v ** pts_to x #0.5R 'v
   ensures pts_to x 'v
   {
     GR.gather x;
@@ -34,7 +50,7 @@ ensures pts_to x #one_half 'v ** regain_half x 'v
 ```pulse //use_regain_half$
 ghost
 fn use_regain_half (x:GR.ref int)
-requires pts_to x #one_half 'v ** regain_half x 'v
+requires pts_to x #0.5R 'v ** regain_half x 'v
 ensures pts_to x 'v
 {
   unfold regain_half;
@@ -44,7 +60,7 @@ ensures pts_to x 'v
 
 //regain_half_q$
 let regain_half_q #a (x:GR.ref a) =
-  forall* u. pts_to x #one_half u @==> pts_to x u 
+  forall* u. pts_to x #0.5R u @==> pts_to x u 
 //regain_half_q$
 
 
@@ -54,11 +70,11 @@ module FA = Pulse.Lib.Forall.Util
 ghost 
 fn intro_regain_half_q (x:GR.ref int)
 requires pts_to x 'v
-ensures pts_to x #one_half 'v ** regain_half_q x
+ensures pts_to x #0.5R 'v ** regain_half_q x
 {
   ghost
   fn aux1 (u:int)
-  requires pts_to x #one_half 'v ** pts_to x #one_half u
+  requires pts_to x #0.5R 'v ** pts_to x #0.5R u
   ensures pts_to x u
   {
     gather x;
@@ -72,18 +88,18 @@ ensures pts_to x #one_half 'v ** regain_half_q x
 ```pulse //use_regain_half_q$
 ghost
 fn use_regain_half_q (x:GR.ref int)
-requires pts_to x #one_half 'u ** regain_half_q x
+requires pts_to x #0.5R 'u ** regain_half_q x
 ensures pts_to x 'u
 {
   unfold regain_half_q;
-  FA.elim #_ #(fun u -> pts_to x #one_half u @==> pts_to x u) 'u;
+  FA.elim #_ #(fun u -> pts_to x #0.5R u @==> pts_to x u) 'u;
   I.elim _ _;
 }
 ```
 
 //can_update$
 let can_update (x:GR.ref int) = 
-  forall* u v. pts_to x #one_half u @==>
+  forall* u v. pts_to x #0.5R u @==>
                pts_to x v
 //can_update$
 
@@ -91,16 +107,16 @@ let can_update (x:GR.ref int) =
 ghost
 fn make_can_update (x:GR.ref int)
 requires pts_to x w
-ensures pts_to x #one_half w ** can_update x
+ensures pts_to x #0.5R w ** can_update x
 {
   ghost
   fn aux (u:int)
-  requires pts_to x #one_half w
-  ensures forall* v. pts_to x #one_half u @==> pts_to x v
+  requires pts_to x #0.5R w
+  ensures forall* v. pts_to x #0.5R u @==> pts_to x v
   {
     ghost
     fn aux (v:int)
-    requires pts_to x #one_half w ** pts_to x #one_half u
+    requires pts_to x #0.5R w ** pts_to x #0.5R u
     ensures pts_to x v
     {
       gather x;
@@ -118,12 +134,12 @@ ensures pts_to x #one_half w ** can_update x
 ```pulse //update$
 ghost
 fn update (x:GR.ref int) (k:int)
-requires pts_to x #one_half 'u ** can_update x
-ensures pts_to x #one_half k ** can_update x
+requires pts_to x #0.5R 'u ** can_update x
+ensures pts_to x #0.5R k ** can_update x
 {
   unfold can_update;
-  FA.elim #_ #(fun u -> forall* v. pts_to x #one_half u @==> pts_to x v) 'u;
-  FA.elim #_ #(fun v -> pts_to x #one_half 'u @==> pts_to x v) k;
+  FA.elim #_ #(fun u -> forall* v. pts_to x #0.5R u @==> pts_to x v) 'u;
+  FA.elim #_ #(fun v -> pts_to x #0.5R 'u @==> pts_to x v) k;
   I.elim _ _;
   make_can_update x;
 }
